InvokeNode and MethodCallTarget
Added a very simple semantics for the InvokeNode and MethodCallTarget
to later replace the CallNode in order to match Graal more closely
and allow programs to be translated fully automatically.

Currently this setup does only handles recursive method calls.

To handle calls to other methods we will need:
1. To match the signature in the MethodCallTargetNode with the name
of a method.
2. An additional input to step_top that maps method signatures to
their IRGraph.

IRNodes.thy
@@ -112,10 +112,11 @@ datatype (discs_sels) IRNode =
   | FixedNode 
   | FixedWithNextNode (ir_next: "SUCC") 
   | FloatingNode 
-  | FrameState (ir_monitorIds: "INPUT_ASSOC list") (ir_outerFrameState_opt: "INPUT_STATE option") (ir_values_opt: "INPUT option list") (ir_virtualObjectMappings_opt: "INPUT_STATE option list") 
+  | FrameState (ir_monitorIds: "INPUT_ASSOC list") (ir_outerFrameState_opt: "INPUT_STATE option") (ir_values_opt: "INPUT list option") (ir_virtualObjectMappings_opt: "INPUT_STATE list option") 
   | IfNode (ir_condition: "INPUT_COND") (ir_trueSuccessor: "SUCC") (ir_falseSuccessor: "SUCC") 
   | IntegerEqualsNode (ir_x: "INPUT") (ir_y: "INPUT") 
   | IntegerLessThanNode (ir_x: "INPUT") (ir_y: "INPUT") 
+  | InvokeNode (ir_callTarget: "INPUT_EXT") (ir_classInit_opt: "INPUT option") (ir_stateDuring_opt: "INPUT_STATE option") (ir_stateAfter_opt: "INPUT_STATE option") (ir_next: "SUCC") 
   | KillingBeginNode (ir_next: "SUCC") 
   | LoadFieldNode (ir_field: string) (ir_object_opt: "INPUT option") (ir_next: "SUCC") 
   | LogicNegationNode (ir_value: "INPUT_COND") 
@@ -123,6 +124,7 @@ datatype (discs_sels) IRNode =
   | LoopEndNode (ir_loopBegin: "INPUT_ASSOC") 
   | LoopExitNode (ir_loopBegin: "INPUT_ASSOC") (ir_stateAfter_opt: "INPUT_STATE option") (ir_next: "SUCC") 
   | MergeNode (ir_ends: "INPUT_ASSOC list") (ir_stateAfter_opt: "INPUT_STATE option") (ir_next: "SUCC") 
+  | MethodCallTargetNode (ir_targetMethod: string) (ir_arguments: "INPUT list") 
   | MulNode (ir_x: "INPUT") (ir_y: "INPUT") 
   | NegateNode (ir_value: "INPUT") 
   | NewArrayNode (ir_length: "INPUT") (ir_stateBefore_opt: "INPUT_STATE option") (ir_next: "SUCC") 
@@ -201,9 +203,9 @@ fun opt_to_list :: "'a option \<Rightarrow> 'a list" where
   "opt_to_list None = []" |
   "opt_to_list (Some v) = [v]"
 
-fun opt_list_to_list :: "'a option list \<Rightarrow> 'a list" where
-  "opt_list_to_list [] = []" |
-  "opt_list_to_list (x # xs) = (opt_to_list x) @ (opt_list_to_list xs)"
+fun opt_list_to_list :: "'a list option \<Rightarrow> 'a list" where
+  "opt_list_to_list None = []" |
+  "opt_list_to_list (Some x) = x"
 
 (* We also define a generic 'inputs_of' for all kinds of nodes. *)
 fun inputs_of :: "IRNode \<Rightarrow> ID list" where
@@ -234,6 +236,7 @@ fun inputs_of :: "IRNode \<Rightarrow> ID list" where
   "inputs_of (IfNode condition trueSuccessor falseSuccessor) = [condition]" |
   "inputs_of (IntegerEqualsNode x y) = [x, y]" |
   "inputs_of (IntegerLessThanNode x y) = [x, y]" |
+  "inputs_of (InvokeNode callTarget classInit stateDuring stateAfter next) = [callTarget] @ (opt_to_list classInit) @ (opt_to_list stateDuring) @ (opt_to_list stateAfter)" |
   "inputs_of (KillingBeginNode next) = []" |
   "inputs_of (LoadFieldNode field object next) = (opt_to_list object)" |
   "inputs_of (LogicNegationNode value) = [value]" |
@@ -241,6 +244,7 @@ fun inputs_of :: "IRNode \<Rightarrow> ID list" where
   "inputs_of (LoopEndNode loopBegin) = [loopBegin]" |
   "inputs_of (LoopExitNode loopBegin stateAfter next) = [loopBegin] @ (opt_to_list stateAfter)" |
   "inputs_of (MergeNode ends stateAfter next) = ends @ (opt_to_list stateAfter)" |
+  "inputs_of (MethodCallTargetNode targetMethod arguments) = arguments" |
   "inputs_of (MulNode x y) = [x, y]" |
   "inputs_of (NegateNode value) = [value]" |
   "inputs_of (NewArrayNode length0 stateBefore next) = [length0] @ (opt_to_list stateBefore)" |
@@ -267,8 +271,8 @@ fun inputs_of :: "IRNode \<Rightarrow> ID list" where
   "inputs_of (RefNode ref) = [ref]" |
   "inputs_of (CallNode startNode arguments succ) = [startNode] @ arguments" 
 
-value "inputs_of (FrameState [4] (Some 3) [Some 5, Some 7] [])"
-value "inputs_of (FrameState [4] None [Some 7] [None, Some 3])"
+value "inputs_of (FrameState [4] (Some 3) (Some [5, 7]) None)"
+value "inputs_of (FrameState [4] None (Some [7]) (Some [3]))"
 
 fun successors_of :: "IRNode \<Rightarrow> ID list" where
   "successors_of (AbsNode value) = []" |
@@ -298,6 +302,7 @@ fun successors_of :: "IRNode \<Rightarrow> ID list" where
   "successors_of (IfNode condition trueSuccessor falseSuccessor) = [trueSuccessor, falseSuccessor]" |
   "successors_of (IntegerEqualsNode x y) = []" |
   "successors_of (IntegerLessThanNode x y) = []" |
+  "successors_of (InvokeNode callTarget classInit stateDuring stateAfter next) = [next]" |
   "successors_of (KillingBeginNode next) = [next]" |
   "successors_of (LoadFieldNode field object next) = [next]" |
   "successors_of (LogicNegationNode value) = []" |
@@ -305,6 +310,7 @@ fun successors_of :: "IRNode \<Rightarrow> ID list" where
   "successors_of (LoopEndNode loopBegin) = []" |
   "successors_of (LoopExitNode loopBegin stateAfter next) = [next]" |
   "successors_of (MergeNode ends stateAfter next) = [next]" |
+  "successors_of (MethodCallTargetNode targetMethod arguments) = []" |
   "successors_of (MulNode x y) = []" |
   "successors_of (NegateNode value) = []" |
   "successors_of (NewArrayNode length0 stateBefore next) = [next]" |
